auto_generated/isabelle/Memory_image.thy
@@ -184,10 +184,10 @@ record symbol_definition
     
 
 
-definition symDefCompare  :: " symbol_definition \<Rightarrow> symbol_definition \<Rightarrow> ordering "  where 
-     " symDefCompare x1 x2 = (        
-(quadrupleCompare (\<lambda> x y. EQ) elf64_symbol_table_entry_compare (genericCompare (op<) (op=)) (genericCompare (op<) (op=)) ((def_symname   x1),(def_syment   x1),(def_sym_scn   x1),(def_sym_idx   x1))
-                ((def_symname   x2),(def_syment   x2),(def_sym_scn   x2),(def_sym_idx   x2))))"
+definition symDefCompare  :: "symbol_definition \<Rightarrow> symbol_definition \<Rightarrow> ordering "  where 
+     " symDefCompare x1 x2 = ((quintupleCompare (\<lambda> x y. stringCompare_method x y)
+        elf64_symbol_table_entry_compare (genericCompare (op<) (op=)) (genericCompare (op<) (op=)) (genericCompare (op<) (op=)) ((def_symname   x1),(def_syment   x1),(def_sym_scn   x1),(def_sym_idx   x1), (def_linkable_idx x1))
+                ((def_symname   x2),(def_syment   x2),(def_sym_scn   x2),(def_sym_idx   x2), (def_linkable_idx x2))))"
 
 
 definition instance_Basic_classes_Ord_Memory_image_symbol_definition_dict  :: "(symbol_definition)Ord_class "  where 
@@ -218,7 +218,7 @@ record symbol_reference
 
 definition symRefCompare  :: " symbol_reference \<Rightarrow> symbol_reference \<Rightarrow> ordering "  where 
      " symRefCompare x1 x2 = (        
-(quadrupleCompare (\<lambda> x y. EQ) elf64_symbol_table_entry_compare (genericCompare (op<) (op=)) (genericCompare (op<) (op=)) ((ref_symname   x1),(ref_syment   x1),(ref_sym_scn   x1),(ref_sym_idx   x1))
+(quadrupleCompare stringCompare_method elf64_symbol_table_entry_compare (genericCompare (op<) (op=)) (genericCompare (op<) (op=)) ((ref_symname   x1),(ref_syment   x1),(ref_sym_scn   x1),(ref_sym_idx   x1))
                 ((ref_symname   x2),(ref_syment   x2),(ref_sym_scn   x2),(ref_sym_idx   x2))))"
 
                 
@@ -272,6 +272,15 @@ datatype reloc_decision = LeaveReloc
                     | ApplyReloc
                     | MakePIC
 
+fun relocDecisionCompare :: "reloc_decision \<Rightarrow> reloc_decision \<Rightarrow> ordering" where
+  "relocDecisionCompare LeaveReloc LeaveReloc = EQ" |
+  "relocDecisionCompare LeaveReloc _ = LT" |
+  "relocDecisionCompare ApplyReloc LeaveReloc = GT" |
+  "relocDecisionCompare ApplyReloc ApplyReloc = EQ" |
+  "relocDecisionCompare ApplyReloc MakePIC = LT" |
+  "relocDecisionCompare MakePIC MakePIC = EQ" |
+  "relocDecisionCompare MakePIC _ = GT"
+
 record symbol_reference_and_reloc_site = 
 
       ref         ::" symbol_reference "
@@ -284,8 +293,8 @@ record symbol_reference_and_reloc_site =
 
 definition symRefAndRelocSiteCompare  :: " symbol_reference_and_reloc_site \<Rightarrow> symbol_reference_and_reloc_site \<Rightarrow> ordering "  where 
      " symRefAndRelocSiteCompare x1 x2 = (        
-(pairCompare symRefCompare (maybeCompare relocSiteCompare) ((ref   x1),(maybe_reloc   x1))
-                ((ref   x2),(maybe_reloc   x2))))"
+(tripleCompare symRefCompare (maybeCompare relocSiteCompare) (maybeCompare (pairCompare relocDecisionCompare (maybeCompare symDefCompare))) ((ref   x1),(maybe_reloc   x1), (maybe_def_bound_to x1))
+                ((ref   x2),(maybe_reloc   x2), (maybe_def_bound_to x2))))"
 
 
 definition instance_Basic_classes_Ord_Memory_image_symbol_reference_and_reloc_site_dict  :: "(symbol_reference_and_reloc_site)Ord_class "  where 
